Heap/MoveUp.v
@@ -5,6 +5,9 @@ Require Import PL.Monad.
 Require Import PL.Monad2.
 Require Import SetsClass.
 Require Import HEAP.Defs.
+Require Import Classical.
+Require Import Coq.Setoids.Setoid.
+Require Import Coq.micromega.Psatz.
 Import SetsNotation
        StateRelMonad
        StateRelMonadOp
@@ -34,6 +37,85 @@ Qed.
 
 (* 有些条件多余 *)
 
+Lemma L2: forall (x y: Z),
+  ~ x <> y -> x = y.
+Proof.
+  intros. tauto.
+Qed.
+
+Lemma L3: forall (bt: BinTree Z Z) (x y1 y2: Z), 
+  BinaryTree.legal bt ->
+    BinaryTree.step_l bt x y1 ->
+      BinaryTree.step_l bt x y2 ->
+        y1 = y2.
+Proof.
+  intros.
+  destruct H.
+  pose proof step_l_unique x y1 y2 H0 H1.
+  tauto.
+Qed.
+
+Lemma L3': forall (bt: BinTree Z Z) (x y1 y2: Z), 
+  BinaryTree.legal bt ->
+    BinaryTree.step_r bt x y1 ->
+      BinaryTree.step_r bt x y2 ->
+        y1 = y2.
+Proof.
+  intros.
+  destruct H.
+  pose proof step_r_unique x y1 y2 H0 H1.
+  tauto.
+Qed.
+
+Lemma L3'': forall (bt: BinTree Z Z) (x y1 y2: Z), 
+  BinaryTree.legal bt ->
+    BinaryTree.step_u bt x y1 ->
+      BinaryTree.step_u bt x y2 ->
+        y1 = y2.
+Proof.
+  intros.
+  destruct H.
+  pose proof step_u_unique x y1 y2 H0 H1.
+  tauto.
+Qed.
+
+Lemma L4: forall (x y: Z),
+  x < y -> x = y -> False.
+Proof. lia. Qed.
+
+Lemma L5: forall (bt: BinTree Z Z) (v fa: Z), 
+  BinaryTree.step_u bt v fa ->
+    BinaryTree.step_l bt v fa ->
+      False.
+Admitted.
+
+Lemma L5': forall (bt: BinTree Z Z) (v fa: Z), 
+  BinaryTree.step_u bt v fa ->
+    BinaryTree.step_r bt v fa ->
+      False.
+Admitted.
+
+Lemma L5'': forall (bt: BinTree Z Z) (v fa: Z), 
+  BinaryTree.step_u bt v fa ->
+    BinaryTree.step_r bt v fa ->
+      False.
+Admitted.
+
+Lemma L6: forall (bt: BinTree Z Z) (x y: Z), 
+  BinaryTree.step_l bt x y ->
+    ~ x = y.
+Admitted.
+
+Lemma L6': forall (bt: BinTree Z Z) (x y: Z), 
+  BinaryTree.step_r bt x y ->
+    ~ x = y.
+Admitted.
+
+Lemma L6'': forall (bt: BinTree Z Z) (x y: Z), 
+  BinaryTree.step_u bt x y ->
+    ~ x = y.
+Admitted.
+
 Fact swap_v_fa_fact1: forall (v fa: Z) (V: Z -> Prop), 
   Hoare
     (fun s => v < fa /\
@@ -47,7 +129,811 @@ Fact swap_v_fa_fact1: forall (v fa: Z) (V: Z -> Prop),
                 Abs s.(heap) V /\
                 BinaryTree.legal s.(heap) /\
                 (Heap s.(heap) \/ Heap_broken_up s.(heap) v)).
-Admitted.
+Proof.
+  unfold Hoare; sets_unfold.
+  unfold Abs.
+  intros.
+  destruct H as [? [[? [? [? ?]]] ?]].
+  split.
+  {
+    unfold swap_v_u in H0.
+    destruct H0 as [? _].
+    apply H0. tauto.
+  }
+  split.
+  {
+    unfold swap_v_u in H0.
+    destruct H0 as [? _].
+    rewrite H0.
+    tauto.
+  }
+  split.
+  {
+    split.
+    {
+      unfold swap_v_u in H0.
+      intros.
+      destruct H0 as [_ ?].
+      pose proof (classic (~ x = v)).
+      pose proof (classic (~ x = fa)).
+      destruct H8, H9.
+      {
+        destruct H0 as [? _].
+        specialize (H0 x H8 H9).
+        pose proof (classic (~ y1 = v)).
+        pose proof (classic (~ y1 = fa)).
+        pose proof (classic (~ y2 = v)).
+        pose proof (classic (~ y2 = fa)).
+        destruct H10, H11, H12, H13.
+        {
+          destruct H0 as [? _].
+
+          pose proof H0 y1 H10 H11.
+          destruct H14 as [[? _] _].
+          apply H14 in H6.
+
+          pose proof H0 y2 H12 H13.
+          destruct H15 as [[? _] _].
+          apply H15 in H7.
+
+          pose proof L3 s1.(heap) x y1 y2 H3 H6 H7.
+          tauto.
+        }
+        {
+          destruct H0 as [? [H0' _]].
+
+          pose proof H0 y1 H10 H11.
+          destruct H14 as [[? _] _].
+          apply H14 in H6.
+
+          destruct H0' as [[? _] _].
+          pose proof L2 y2 fa H13.
+          subst y2.
+          apply H15 in H7.
+          
+          pose proof L3 s1.(heap) x y1 v H3 H6 H7.
+          tauto.
+        }
+        {
+          destruct H0 as [? [_ H0']].
+
+          pose proof H0 y1 H10 H11.
+          destruct H14 as [[? _] _].
+          apply H14 in H6.
+
+          destruct H0' as [[? _] _].
+          pose proof L2 y2 v H12.
+          subst y2.
+          apply H15 in H7.
+
+          pose proof L3 s1.(heap) x y1 fa H3 H6 H7.
+          tauto.
+        }
+        {
+          lia.
+        }
+        {
+          destruct H0 as [? [H0' _]].
+
+          destruct H0' as [[? _] _].
+          pose proof L2 y1 fa H11.
+          subst y1.
+          apply H14 in H6.
+
+          pose proof H0 y2 H12 H13.
+          destruct H15 as [[? _] _].
+          apply H15 in H7.
+          
+          pose proof L3 s1.(heap) x v y2 H3 H6 H7.
+          lia.
+        }
+        {
+          lia.
+        }
+        {
+          destruct H0 as [_ [H0 H0']].
+
+          destruct H0 as [[? _] _].
+          pose proof L2 y1 fa H11.
+          subst y1.
+          apply H0 in H6.
+
+          destruct H0' as [[? _] _].
+          pose proof L2 y2 v H12.
+          subst y2.
+          apply H14 in H7.
+
+          pose proof L3 s1.(heap) x v fa H3 H6 H7.
+          lia.
+        }
+        {
+          lia.
+        }
+        {
+          destruct H0 as [H0 [_ H0']].
+
+          destruct H0' as [[? _] _].
+          pose proof L2 y1 v H10.
+          subst y1.
+          apply H14 in H6.
+
+          pose proof H0 y2 H12 H13.
+          destruct H15 as [[? _] _].
+          apply H15 in H7.
+
+          pose proof L3 s1.(heap) x fa y2 H3 H6 H7.
+          lia.
+        }
+        {
+          destruct H0 as [_ [H0 H0']].
+
+          destruct H0' as [[? _] _].
+          pose proof L2 y1 v H10.
+          subst y1.
+          apply H14 in H6.
+
+          destruct H0 as [[? _] _].
+          pose proof L2 y2 fa H13.
+          subst y2.
+          apply H0 in H7.
+
+          pose proof L3 s1.(heap) x fa v H3 H6 H7.
+          lia.
+        }
+        {
+          lia.
+        }
+        {
+          lia.
+        }
+        {
+          lia.
+        }
+        {
+          lia.
+        }
+        {
+          lia.
+        }
+        {
+          lia.
+        }
+      }
+      {
+        destruct H0 as [_ [? _]].
+        pose proof L2 x fa H9.
+        subst x.
+        pose proof (classic (~ y1 = v)).
+        pose proof (classic (~ y2 = v)).
+        destruct H10, H11.
+        {
+          destruct H0 as [? _].
+
+          pose proof H0 y1 H10.
+          destruct H12 as [[? _] _].
+          apply H12 in H6.
+
+          pose proof H0 y2 H11.
+          destruct H13 as [[? _] _].
+          apply H13 in H7.
+
+          pose proof L3 s1.(heap) v y1 y2 H3 H6 H7.
+          tauto.
+        }
+        {
+          destruct H0 as [_ ?].
+
+          destruct H0 as [[? _] _].
+          pose proof L2 y2 v H11.
+          subst y2.
+          apply H0 in H7.
+          
+          pose proof L5 s1.(heap) v fa H5 H7.
+          tauto.
+        }
+        {
+          destruct H0 as [_ ?].
+
+          destruct H0 as [[? _] _].
+          pose proof L2 y1 v H10.
+          subst y1.
+          apply H0 in H6.
+          
+          pose proof L5 s1.(heap) v fa H5 H6.
+          tauto.
+        }
+        {
+          lia.
+        }
+      }
+      {
+        destruct H0 as [_ [_ ?]].
+        pose proof L2 x v H8.
+        subst x.
+        pose proof (classic (~ y1 = fa)).
+        pose proof (classic (~ y2 = fa)).
+        destruct H10, H11.
+        {
+          destruct H0 as [? _].
+
+          pose proof H0 y1 H10.
+          destruct H12 as [[? _] _].
+          apply H12 in H6.
+
+          pose proof H0 y2 H11.
+          destruct H13 as [[? _] _].
+          apply H13 in H7.
+
+          pose proof L3 s1.(heap) fa y1 y2 H3 H6 H7.
+          tauto.
+        }
+        {
+          destruct H0 as [H0 H0'].
+
+          pose proof L6 s2.(heap) v y1 H6.
+          pose proof H0 y1 H10.
+          destruct H13 as [[? _] _].
+          apply H13 in H6.
+
+          destruct H0' as [[? _] _].
+          pose proof L2 y2 fa H11.
+          subst y2.
+          apply H14 in H7.
+          
+          pose proof L3 s1.(heap) fa y1 v H3 H6 H7.
+          lia.
+        }
+        {
+          destruct H0 as [H0 H0'].
+
+          destruct H0' as [[? _] _].
+          pose proof L2 y1 fa H10.
+          subst y1.
+          apply H12 in H6.
+
+          pose proof L6 s2.(heap) v y2 H7.
+          pose proof H0 y2 H11.
+          destruct H14 as [[? _] _].
+          apply H14 in H7.   
+          
+          pose proof L3 s1.(heap) fa v y2 H3 H6 H7.
+          lia.
+        }
+        {
+          lia. 
+        }
+      }
+      {
+        lia.
+      }
+    }
+    {
+      unfold swap_v_u in H0.
+      intros.
+      destruct H0 as [_ ?].
+      pose proof (classic (~ x = v)).
+      pose proof (classic (~ x = fa)).
+      destruct H8, H9.
+      {
+        destruct H0 as [? _].
+        specialize (H0 x H8 H9).
+        pose proof (classic (~ y1 = v)).
+        pose proof (classic (~ y1 = fa)).
+        pose proof (classic (~ y2 = v)).
+        pose proof (classic (~ y2 = fa)).
+        destruct H10, H11, H12, H13.
+        {
+          destruct H0 as [? _].
+
+          pose proof H0 y1 H10 H11.
+          destruct H14 as [_ [? _]].
+          apply H14 in H6.
+
+          pose proof H0 y2 H12 H13.
+          destruct H15 as [_ [? _]].
+          apply H15 in H7.
+
+          pose proof L3' s1.(heap) x y1 y2 H3 H6 H7.
+          tauto.
+        }
+        {
+          destruct H0 as [? [H0' _]].
+
+          pose proof H0 y1 H10 H11.
+          destruct H14 as [_ [? _]].
+          apply H14 in H6.
+
+          destruct H0' as [_ [? _]].
+          pose proof L2 y2 fa H13.
+          subst y2.
+          apply H15 in H7.
+          
+          pose proof L3' s1.(heap) x y1 v H3 H6 H7.
+          tauto.
+        }
+        {
+          destruct H0 as [? [_ H0']].
+
+          pose proof H0 y1 H10 H11.
+          destruct H14 as [_ [? _]].
+          apply H14 in H6.
+
+          destruct H0' as [_ [? _]].
+          pose proof L2 y2 v H12.
+          subst y2.
+          apply H15 in H7.
+
+          pose proof L3' s1.(heap) x y1 fa H3 H6 H7.
+          tauto.
+        }
+        {
+          lia.
+        }
+        {
+          destruct H0 as [? [H0' _]].
+
+          destruct H0' as [_ [? _]].
+          pose proof L2 y1 fa H11.
+          subst y1.
+          apply H14 in H6.
+
+          pose proof H0 y2 H12 H13.
+          destruct H15 as [_ [? _]].
+          apply H15 in H7.
+          
+          pose proof L3' s1.(heap) x v y2 H3 H6 H7.
+          lia.
+        }
+        {
+          lia.
+        }
+        {
+          destruct H0 as [_ [H0 H0']].
+
+          destruct H0 as [_ [? _]].
+          pose proof L2 y1 fa H11.
+          subst y1.
+          apply H0 in H6.
+
+          destruct H0' as [_ [? _]].
+          pose proof L2 y2 v H12.
+          subst y2.
+          apply H14 in H7.
+
+          pose proof L3' s1.(heap) x v fa H3 H6 H7.
+          lia.
+        }
+        {
+          lia.
+        }
+        {
+          destruct H0 as [H0 [_ H0']].
+
+          destruct H0' as [_ [? _]].
+          pose proof L2 y1 v H10.
+          subst y1.
+          apply H14 in H6.
+
+          pose proof H0 y2 H12 H13.
+          destruct H15 as [_ [? _]].
+          apply H15 in H7.
+
+          pose proof L3' s1.(heap) x fa y2 H3 H6 H7.
+          lia.
+        }
+        {
+          destruct H0 as [_ [H0 H0']].
+
+          destruct H0' as [_ [? _]].
+          pose proof L2 y1 v H10.
+          subst y1.
+          apply H14 in H6.
+
+          destruct H0 as [_ [? _]].
+          pose proof L2 y2 fa H13.
+          subst y2.
+          apply H0 in H7.
+
+          pose proof L3' s1.(heap) x fa v H3 H6 H7.
+          lia.
+        }
+        {
+          lia.
+        }
+        {
+          lia.
+        }
+        {
+          lia.
+        }
+        {
+          lia.
+        }
+        {
+          lia.
+        }
+        {
+          lia.
+        }
+      }
+      {
+        destruct H0 as [_ [? _]].
+        pose proof L2 x fa H9.
+        subst x.
+        pose proof (classic (~ y1 = v)).
+        pose proof (classic (~ y2 = v)).
+        destruct H10, H11.
+        {
+          destruct H0 as [? _].
+
+          pose proof H0 y1 H10.
+          destruct H12 as [_ [? _]].
+          apply H12 in H6.
+
+          pose proof H0 y2 H11.
+          destruct H13 as [_ [? _]].
+          apply H13 in H7.
+
+          pose proof L3' s1.(heap) v y1 y2 H3 H6 H7.
+          tauto.
+        }
+        {
+          destruct H0 as [_ ?].
+
+          destruct H0 as [_ [? _]].
+          pose proof L2 y2 v H11.
+          subst y2.
+          apply H0 in H7.
+          
+          pose proof L5' s1.(heap) v fa H5 H7.
+          tauto.
+        }
+        {
+          destruct H0 as [_ ?].
+
+          destruct H0 as [_ [? _]].
+          pose proof L2 y1 v H10.
+          subst y1.
+          apply H0 in H6.
+          
+          pose proof L5' s1.(heap) v fa H5 H6.
+          tauto.
+        }
+        {
+          lia.
+        }
+      }
+      {
+        destruct H0 as [_ [_ ?]].
+        pose proof L2 x v H8.
+        subst x.
+        pose proof (classic (~ y1 = fa)).
+        pose proof (classic (~ y2 = fa)).
+        destruct H10, H11.
+        {
+          destruct H0 as [? _].
+
+          pose proof H0 y1 H10.
+          destruct H12 as [_ [? _]].
+          apply H12 in H6.
+
+          pose proof H0 y2 H11.
+          destruct H13 as [_ [? _]].
+          apply H13 in H7.
+
+          pose proof L3' s1.(heap) fa y1 y2 H3 H6 H7.
+          tauto.
+        }
+        {
+          destruct H0 as [H0 H0'].
+
+          pose proof L6' s2.(heap) v y1 H6.
+          pose proof H0 y1 H10.
+          destruct H13 as [_ [? _]].
+          apply H13 in H6.
+
+          destruct H0' as [_ [? _]].
+          pose proof L2 y2 fa H11.
+          subst y2.
+          apply H14 in H7.
+          
+          pose proof L3' s1.(heap) fa y1 v H3 H6 H7.
+          lia.
+        }
+        {
+          destruct H0 as [H0 H0'].
+
+          destruct H0' as [_ [? _]].
+          pose proof L2 y1 fa H10.
+          subst y1.
+          apply H12 in H6.
+
+          pose proof L6' s2.(heap) v y2 H7.
+          pose proof H0 y2 H11.
+          destruct H14 as [_ [? _]].
+          apply H14 in H7.   
+          
+          pose proof L3' s1.(heap) fa v y2 H3 H6 H7.
+          lia.
+        }
+        {
+          lia. 
+        }
+      }
+      {
+        lia.
+      }
+    }
+    {
+      unfold swap_v_u in H0.
+      intros.
+      destruct H0 as [_ ?].
+      pose proof (classic (~ x = v)).
+      pose proof (classic (~ x = fa)).
+      destruct H8, H9.
+      {
+        destruct H0 as [? _].
+        specialize (H0 x H8 H9).
+        pose proof (classic (~ y1 = v)).
+        pose proof (classic (~ y1 = fa)).
+        pose proof (classic (~ y2 = v)).
+        pose proof (classic (~ y2 = fa)).
+        destruct H10, H11, H12, H13.
+        {
+          destruct H0 as [? _].
+
+          pose proof H0 y1 H10 H11.
+          destruct H14 as [_ [_ ?]].
+          apply H14 in H6.
+
+          pose proof H0 y2 H12 H13.
+          destruct H15 as [_ [_ ?]].
+          apply H15 in H7.
+
+          pose proof L3'' s1.(heap) x y1 y2 H3 H6 H7.
+          tauto.
+        }
+        {
+          destruct H0 as [? [H0' _]].
+
+          pose proof H0 y1 H10 H11.
+          destruct H14 as [_ [_ ?]].
+          apply H14 in H6.
+
+          destruct H0' as [_ [_ ?]].
+          pose proof L2 y2 fa H13.
+          subst y2.
+          apply H15 in H7.
+          
+          pose proof L3'' s1.(heap) x y1 v H3 H6 H7.
+          tauto.
+        }
+        {
+          destruct H0 as [? [_ H0']].
+
+          pose proof H0 y1 H10 H11.
+          destruct H14 as [_ [_ ?]].
+          apply H14 in H6.
+
+          destruct H0' as [_ [_ ?]].
+          pose proof L2 y2 v H12.
+          subst y2.
+          apply H15 in H7.
+
+          pose proof L3'' s1.(heap) x y1 fa H3 H6 H7.
+          tauto.
+        }
+        {
+          lia.
+        }
+        {
+          destruct H0 as [? [H0' _]].
+
+          destruct H0' as [_ [_ ?]].
+          pose proof L2 y1 fa H11.
+          subst y1.
+          apply H14 in H6.
+
+          pose proof H0 y2 H12 H13.
+          destruct H15 as [_ [_ ?]].
+          apply H15 in H7.
+          
+          pose proof L3'' s1.(heap) x v y2 H3 H6 H7.
+          lia.
+        }
+        {
+          lia.
+        }
+        {
+          destruct H0 as [_ [H0 H0']].
+
+          destruct H0 as [_ [_ ?]].
+          pose proof L2 y1 fa H11.
+          subst y1.
+          apply H0 in H6.
+
+          destruct H0' as [_ [_ ?]].
+          pose proof L2 y2 v H12.
+          subst y2.
+          apply H14 in H7.
+
+          pose proof L3'' s1.(heap) x v fa H3 H6 H7.
+          lia.
+        }
+        {
+          lia.
+        }
+        {
+          destruct H0 as [H0 [_ H0']].
+
+          destruct H0' as [_ [_ ?]].
+          pose proof L2 y1 v H10.
+          subst y1.
+          apply H14 in H6.
+
+          pose proof H0 y2 H12 H13.
+          destruct H15 as [_ [_ ?]].
+          apply H15 in H7.
+
+          pose proof L3'' s1.(heap) x fa y2 H3 H6 H7.
+          lia.
+        }
+        {
+          destruct H0 as [_ [H0 H0']].
+
+          destruct H0' as [_ [_ ?]].
+          pose proof L2 y1 v H10.
+          subst y1.
+          apply H14 in H6.
+
+          destruct H0 as [_ [_ ?]].
+          pose proof L2 y2 fa H13.
+          subst y2.
+          apply H0 in H7.
+
+          pose proof L3'' s1.(heap) x fa v H3 H6 H7.
+          lia.
+        }
+        {
+          lia.
+        }
+        {
+          lia.
+        }
+        {
+          lia.
+        }
+        {
+          lia.
+        }
+        {
+          lia.
+        }
+        {
+          lia.
+        }
+      }
+      {
+        destruct H0 as [_ [? _]].
+        pose proof L2 x fa H9.
+        subst x.
+        pose proof (classic (~ y1 = v)).
+        pose proof (classic (~ y2 = v)).
+        destruct H10, H11.
+        {
+          destruct H0 as [? _].
+
+          pose proof H0 y1 H10.
+          destruct H12 as [_ [_ ?]].
+          apply H12 in H6.
+
+          pose proof H0 y2 H11.
+          destruct H13 as [_ [_ ?]].
+          apply H13 in H7.
+
+          pose proof L3'' s1.(heap) v y1 y2 H3 H6 H7.
+          tauto.
+        }
+        {
+          destruct H0 as [H0 H0'].
+
+          pose proof L6'' s2.(heap) fa y1 H6.
+          pose proof H0 y1 H10.
+          destruct H13 as [_ [_ ?]].
+          apply H13 in H6.
+
+          destruct H0' as [_ [_ ?]].
+          pose proof L2 y2 v H11.
+          subst y2.
+          apply H14 in H7.
+          
+          pose proof L3'' s1.(heap) v y1 fa H3 H6 H7.
+          lia.
+        }
+        {
+          destruct H0 as [H0 H0'].
+
+          destruct H0' as [_ [_ ?]].
+          pose proof L2 y1 v H10.
+          subst y1.
+          apply H12 in H6.
+
+          pose proof L6'' s2.(heap) fa y2 H7.
+          pose proof H0 y2 H11.
+          destruct H14 as [_ [_ ?]].
+          apply H14 in H7.
+
+          pose proof L3'' s1.(heap) v fa y2 H3 H6 H7.
+          lia.
+        }
+        {
+          lia.
+        }
+      }
+      {
+        destruct H0 as [_ [_ ?]].
+        pose proof L2 x v H8.
+        subst x.
+        pose proof (classic (~ y1 = fa)).
+        pose proof (classic (~ y2 = fa)).
+        destruct H10, H11.
+        {
+          destruct H0 as [? _].
+
+          pose proof H0 y1 H10.
+          destruct H12 as [_ [_ ?]].
+          apply H12 in H6.
+
+          pose proof H0 y2 H11.
+          destruct H13 as [_ [_ ?]].
+          apply H13 in H7.
+
+          pose proof L3'' s1.(heap) fa y1 y2 H3 H6 H7.
+          tauto.
+        }
+        {
+          destruct H0 as [H0 H0'].
+
+          pose proof L6'' s2.(heap) v y1 H6.
+          pose proof H0 y1 H10.
+          destruct H13 as [_ [_ ?]].
+          apply H13 in H6.
+
+          destruct H0' as [_ [_ ?]].
+          pose proof L2 y2 fa H11.
+          subst y2.
+          apply H14 in H7.
+          
+          pose proof L3'' s1.(heap) fa y1 v H3 H6 H7.
+          lia.
+        }
+        {
+          destruct H0 as [H0 H0'].
+
+          destruct H0' as [_ [_ ?]].
+          pose proof L2 y1 fa H10.
+          subst y1.
+          apply H12 in H6.
+
+          pose proof L6'' s2.(heap) v y2 H7.
+          pose proof H0 y2 H11.
+          destruct H14 as [_ [_ ?]].
+          apply H14 in H7.   
+          
+          pose proof L3'' s1.(heap) fa v y2 H3 H6 H7.
+          lia.
+        }
+        {
+          lia. 
+        }
+      }
+      {
+        lia.
+      }
+    }
+  }
+
+
 
 
 Lemma L1: forall (x y: Z),
